# Mechanical Systems Notes
## Symbols
|Symbol|Name|Unit|
|---|---|---|
|$a$|Acceleration|$ms^{-2}$ (Metres per second per second)|
|$\alpha$|Angular acceleration|$rads^{-2}$ (Radians per second per second)|
|$d$|Distance|$m$ (Metres)|
|$E$|Energy|$J$ (Joules)|
|$E_k$|Kinetic energy|&uarr;
|$E_p$|Potential energy|&uarr;
|$f$|Frequency|Hz (Hertz)|
|$F$|Force|$N$ (Newtons)|
|$F_c$|Centripetal force| &uarr;
|$I$|Moment of Inertia|$kgm^2$ (kKilogram metres squared)|
|$k$|Spring constant|$Nm^{-1}$ (Newtons per metre)|
|$l$|Length|$m$ (Metres)|
|$L$|Angular momentum|$kgm^2s^{-1}$ (Kilogram meters squared per second)|
|$m$|Mass|$kg$ (Kilograms)|
|$M$|Moment of force|$Nm$ (Newton meters)|
|$p$|Momentum|$kgms^{-1}$ (Kilograms per meter per second)|
|$t$|Time|$s$ (Seconds)|
|$T$|Interval of time|&uarr;
|$\tau$|Torque|$Nm$ (Newton metres)|
|$v$|Velocity|$ms^{-1}$ (Metres per second)|
|$\omega$|Angular velocity|$rads^{-1}$ (Radians per second)|




## Constants
|Symbol|Name|Value|
|---|---|---|
|$G$|Gravitational constant|$9.81ms^{-1}$|


## Equations
### Standard
- $E_{K(LIN)} = \frac{1}{2}mv^2$
- $E_p = \frac{1}{2}ky^2$
- $\Delta E_p = mg \Delta h$
- $F = ma$
- $F = -ky$
- $\Delta p = F \Delta t$
- $T = 2 \pi \sqrt{\frac{l}{g}}$
- $W = Fd$
- $x_{COM} = \frac{m_1 x_1 + m_2 + x_2}{m_1 + m_2}$
- $y = A sin \omega t$
- $y = A cos \omega t$

### Rotational
- $a = -A \omega^2 sin \omega t$
- $a = -A \omega^2 cos \omega t$
- $a = r \alpha$
- $a = - \omega^2 y$
- $\alpha = \frac{\Delta \omega}{\Delta t}$
- $d = r\theta$
- $E_{K(ROT)} = \frac{1}{2} I \omega^2$
- $F_g = \frac{GMm}{r^2}$
- $F_c = \frac{mv^2}{r}$
- $I = mr^2$ (For hollow ring)
- $I = \frac{1}{2}mr^2$ (For solid disk)
- $I = \frac{2}{5}mr^2$ (For solid sphere)
- $L = mvr$
- $L = mr^2 \frac{v}{r}$
- $L = I \omega$
- $T = 2 \pi \sqrt{\frac{m}{k}}$
- $\tau = I\alpha$
- $\tau = Fr$
- $\tau = r F cos \theta$
- $v = A \omega cos \omega t$
- $v = -A \omega sin \omega t$
- $v \geq \sqrt{gr}$
- $\omega = 2 \pi f$
- $\omega_f = \omega_i + \alpha t$
- $\omega = \frac{\Delta \theta}{\Delta t}$
- $\omega_f^2 = \omega_i^2 + 2 \alpha \theta$
- $\theta = \omega_i t + \frac{1}{2} \alpha t^2$
- $\theta = \omega_f t - \frac{1}{2} \alpha t^2$
- $\theta = \frac{\omega_f + \omega_i}{2}t$

### Kinematics


